Finish up PHOAS-interaction

src/Assembly/Equivalence.v
@@ -13,6 +13,7 @@ Require Import Crypto.Stringification.Language.
 Require Import Crypto.Util.Strings.Show.
 Require Import Crypto.Util.Option.
 Require Import Crypto.Util.OptionList.
+Require Import Crypto.Util.Notations.
 Import API.Compilers APINotations.Compilers AbstractInterpretation.ZRange.Compilers.
 Import ListNotations.
 Local Open Scope string_scope.
@@ -65,27 +66,20 @@ include enough information in the error message to generate .dot files
 of the equivalence graphs.  If desired, we can parameterize the error
 printing functions on command-lines options indicating how verbose to
 be in printing the error message. *)
-Inductive BoundsDataError :=
-| Unknown_array_length (t : base.type)
-| Invalid_arrow_type (t : API.type)
-.
 Inductive EquivalenceCheckingError :=
 | Could_not_prove_equivalence
 | Not_enough_registers (num_given num_extra_needed : nat)
-| Invalid_bounds_data (e : BoundsDataError)
 | Incorrect_array_input_dag_node
 | Incorrect_Z_input_dag_node
-| Not_enough_input_dag_nodes (t : Compilers.type.type base.type)
-| Invalid_input_type (t : Compilers.type.type base.type)
+| Not_enough_input_dag_nodes (t : API.type)
+| Unknown_array_length (t : base.type)
+| Invalid_arrow_type (t : API.type)
+| Invalid_argument_type (t : API.type)
+| Invalid_higher_order_application {var} {s d : API.type} (f : API.expr (var:=var) (s -> d)) (x : API.expr (var:=var) s)
+| Invalid_higher_order_let {var} {s : API.type} (x : API.expr (var:=var) s)
+| Unhandled_identifier {t} (idc : ident t)
 .
 
-Global Instance show_lines_BoundsDataError : ShowLines BoundsDataError
-  := fun err => match err with
-                | Unknown_array_length t => ["Unknown array length of type " ++ show t ++ "."]%string
-                | Invalid_arrow_type t => ["Invalid higher order function involving the type " ++ show t ++ "."]%string
-                end%list.
-Global Instance show_BoundsDataError : Show BoundsDataError
-  := fun err => String.concat String.NewLine (show_lines err).
 Global Instance show_lines_EquivalenceCheckingError : ShowLines EquivalenceCheckingError
   := fun err => match err with
                 | Could_not_prove_equivalence
@@ -98,31 +92,59 @@ Global Instance show_lines_EquivalenceCheckingError : ShowLines EquivalenceCheck
                   => ["Internal error: Input dag node had an unexpected Z."]
                 | Not_enough_input_dag_nodes t
                   => ["Internal error: Not enough input dag nodes to allocate for type " ++ show t ++ "."]%string
-                | Invalid_input_type t
-                  => ["Invalid type for input argument " ++ show t ++ "."]%string
-                | Invalid_bounds_data err
-                  => show_lines err
+                | Invalid_argument_type t
+                  => ["Invalid type for argument: " ++ show t]%string
+                | Unknown_array_length t => ["Unknown array length of type " ++ show t ++ "."]%string
+                | Invalid_arrow_type t => ["Invalid higher order function involving the type " ++ show t ++ "."]%string
+                | Invalid_higher_order_application var s d f x
+                  => let __ := @Compilers.ToString.PHOAS.expr.partially_show_expr in
+                     ["Invalid higher-order application node with argument of type " ++ show s ++ ":"
+                      ; "Function expression: " ++ show f
+                      ; "Argument expression: " ++ show x]%string
+                | Invalid_higher_order_let var s x
+                  => let __ := @Compilers.ToString.PHOAS.expr.partially_show_expr in
+                     ["Invalid higher-order let-in node with argument of type " ++ show s ++ ":"
+                      ; "Let-bound expression: " ++ show x]%string
+                | Unhandled_identifier t idc
+                  => ["Identifier not yet handled by symbolic evaluation: " ++ show idc ++ "."]%string
                 end%list.
 Global Instance show_EquivalenceCheckingError : Show EquivalenceCheckingError
   := fun err => String.concat String.NewLine (show_lines err).
 
-(** FIXME: remove axioms *)
+(** FIXME: pick better definitions *)
 Definition symbol := N.
 Definition gensym_state := N.
 Definition gensym_state_init : gensym_state := 0%N.
 Definition gensym (st : gensym_state) : symbol * gensym_state := (st, N.succ st).
 Definition idx := N.
-Axiom dag : Type.
-Axiom empty_dag : dag.
-Axiom merge : symbol -> dag -> idx * dag.
-Axiom merge_literal : Z -> dag -> idx * dag.
+Definition dummy_dag : { T : Type & T }. exists unit; constructor. Qed.
+(*Axiom*) Definition dag : Type := projT1 dummy_dag.
+(*Axiom*) Definition empty_dag : dag := projT2 dummy_dag.
+(*Axiom*) Definition merge : symbol -> dag -> idx * dag := fun _ st => (0%N, st).
+(*Axiom*) Definition merge_literal : Z -> dag -> idx * dag := fun _ st => (0%N, st).
 
-Definition input_type_spec := list (option nat). (* list of array lengths; None means not an array *)
+(** symbolic evaluations live in the state monad, pushed to the leaves of a PHOAS type *)
+Definition symexM T := dag -> ErrorT EquivalenceCheckingError (T * dag).
+Definition symex_return {T} (v : T) : symexM T := fun st => Success (v, st).
+Definition symex_error {T} err : symexM T := fun st => Error err.
+Definition symex_bind {A B} (v : symexM A) (f : A -> symexM B) : symexM B
+  := fun st => (v <- v st; let '(a, st) := v in f a st)%error.
+Delimit Scope symex_scope with symex.
+Bind Scope symex_scope with symexM.
+Notation "'slet' x .. y <- X ; B"  := (symex_bind X (fun x => .. (fun y => B%symex) .. )) : symex_scope.
+Notation "A <- X ; B" := (symex_bind X (fun A => B%symex)) : symex_scope.
+(* light alias *)
+Definition merge_literalM (v : Z) : symexM idx := fun st => Success (merge_literal v st).
+
+(** FIXME: change *)
+Definition merge_addition : idx -> idx -> symexM idx := fun _ _ st => Error (Unhandled_identifier ident.Z_add).
+
+Definition type_spec := list (option nat). (* list of array lengths; None means not an array *)
 
 (** Convert PHOAS info about types and argument bounds into a simplified specification *)
 Fixpoint simplify_base_type
          (t : base.type)
-  : forall arg_bounds : ZRange.type.base.option.interp t, ErrorT EquivalenceCheckingError input_type_spec
+  : forall arg_bounds : ZRange.type.base.option.interp t, ErrorT EquivalenceCheckingError type_spec
   := match t return ZRange.type.base.option.interp t -> _ with
      | base.type.unit
        => fun 'tt => Success []
@@ -136,24 +158,24 @@ Fixpoint simplify_base_type
      | base.type.list (base.type.type_base base.type.Z)
        => fun b
           => match b with
-             | None => Error (Invalid_bounds_data (Unknown_array_length t))
+             | None => Error (Unknown_array_length t)
              | Some bs => Success [Some (List.length bs)]
              end
      | base.type.type_base _
      | base.type.option _
      | base.type.list _
-       => fun _ => Error (Invalid_input_type (type.base t))
+       => fun _ => Error (Invalid_argument_type (type.base t))
      end%error.
 Definition simplify_type
-         (t : Compilers.type.type base.type)
-  : forall arg_bounds : ZRange.type.option.interp t, ErrorT EquivalenceCheckingError input_type_spec
+         (t : API.type)
+  : forall arg_bounds : ZRange.type.option.interp t, ErrorT EquivalenceCheckingError type_spec
   := match t with
      | type.base t => simplify_base_type t
-     | type.arrow _ _ => fun _ => Error (Invalid_input_type t)
+     | type.arrow _ _ => fun _ => Error (Invalid_argument_type t)
      end.
 Fixpoint simplify_input_type
-         (t : Compilers.type.type base.type)
-  : forall arg_bounds : type.for_each_lhs_of_arrow ZRange.type.option.interp t, ErrorT EquivalenceCheckingError input_type_spec
+         (t : API.type)
+  : forall arg_bounds : type.for_each_lhs_of_arrow ZRange.type.option.interp t, ErrorT EquivalenceCheckingError type_spec
   := match t return type.for_each_lhs_of_arrow ZRange.type.option.interp t -> _ with
      | type.base _ => fun 'tt => Success []
      | type.arrow A B
@@ -163,7 +185,7 @@ Fixpoint simplify_input_type
              Success (vA ++ vB))
      end%error.
 
-Fixpoint build_inputs (st : dag * gensym_state) (types : input_type_spec) : list (idx + list idx) * (dag * gensym_state)
+Fixpoint build_inputs (st : dag * gensym_state) (types : type_spec) : list (idx + list idx) * (dag * gensym_state)
   := match types with
      | [] => ([], st)
      | None :: tys
@@ -185,7 +207,7 @@ Fixpoint build_inputs (st : dag * gensym_state) (types : input_type_spec) : list
           (inr idxs :: rest, (d, st))
      end.
 
-(** PHOAS var type, storing dag indices *)
+(** PHOAS var type, storing dag indices or nat literals *)
 Fixpoint base_var (t : base.type) : Set
   := match t with
      | base.type.unit
@@ -193,11 +215,13 @@ Fixpoint base_var (t : base.type) : Set
      | base.type.type_base base.type.Z => idx
      | base.type.prod A B => base_var A * base_var B
      | base.type.list A => list (base_var A)
+     | base.type.type_base base.type.nat => nat
+     | base.type.type_base base.type.zrange => ZRange.zrange
      | base.type.type_base _
      | base.type.option _
        => unit (* should not happen *)
      end.
-Definition var (t : Compilers.type.type base.type) : Set
+Definition var (t : API.type) : Set
   := match t with
      | type.base t => base_var t
      | type.arrow s d => Empty_set
@@ -231,15 +255,15 @@ Fixpoint build_base_var (t : base.type) (indices : list (idx + list idx))
      | base.type.type_base _, _
      | base.type.option _, _
      | base.type.list _, _ :: _
-       => Error (Invalid_input_type (type.base t))
+       => Error (Invalid_argument_type (type.base t))
      end%error.
-Definition build_var (t : Compilers.type.type base.type) (indices : list (idx + list idx))
+Definition build_var (t : API.type) (indices : list (idx + list idx))
   : ErrorT EquivalenceCheckingError (var t * list (idx + list idx))
   := match t with
      | type.base t => build_base_var t indices
-     | type.arrow _ _ => Error (Invalid_input_type t)
+     | type.arrow _ _ => Error (Invalid_argument_type t)
      end.
-Fixpoint build_input_var (t : Compilers.type.type base.type) (indices : list (idx + list idx))
+Fixpoint build_input_var (t : API.type) (indices : list (idx + list idx))
   : ErrorT EquivalenceCheckingError (type.for_each_lhs_of_arrow var t * list (idx + list idx))
   := match t with
      | type.base _ => Success (tt, indices)
@@ -251,68 +275,208 @@ Fixpoint build_input_var (t : Compilers.type.type base.type) (indices : list (id
           Success ((vA, vB), indices))
      end%error.
 
-(** symbolic evaluations live in the state monad, pushed to the leaves of a PHOAS type *)
-Definition symexM T := dag -> ErrorT EquivalenceCheckingError (T * dag).
-(* light alias *)
-Definition merge_literalM (v : Z) : symexM idx := fun st => Success (merge_literal v st).
-Fixpoint symex_T (t : Compilers.type.type base.type) : Type
+(** Symbolic evaluation does not support higher-order functions *)
+Fixpoint symex_T (t : API.type) : Type
   := match t with
      | type.base t => symexM (base_var t)
      | type.arrow s d
-       => ErrorT EquivalenceCheckingError (symex_T s -> symex_T d)
+       => match s with
+          | type.base s => base_var s
+          | type.arrow _ _ => Empty_set
+          end -> symex_T d
      end.
-Definition symex_return {T} (v : T) : symexM T := fun st => Success (v, st).
-Definition symex_bind {A B} (v : symexM A) (f : A -> symexM B) : symexM B
-  := fun st => (v <- v st; let '(a, st) := v in f a st)%error.
-Definition symex_T_return {t : Compilers.type.type base.type} : var t -> symex_T t
+Definition symex_T_return {t : API.type} : var t -> symex_T t
   := match t return var t -> symex_T t with
      | type.base t => symex_return
      | type.arrow s d
        => fun f : Empty_set => match f with end
      end.
-Delimit Scope symex_scope with symex.
-Bind Scope symex_scope with symexM.
+Fixpoint symex_T_error {t} err : symex_T t
+  := match t return symex_T t with
+     | type.base t => symex_error err
+     | type.arrow s d => fun _ => @symex_T_error d err
+     end.
+Fixpoint symex_T_bind_base {T t} : symexM T -> (T -> symex_T t) -> symex_T t
+  := match t with
+     | type.base _ => symex_bind
+     | type.arrow s d
+       => fun v f x => @symex_T_bind_base T d v (fun w => f w x)
+     end.
 Bind Scope symex_scope with symex_T.
-(** TODO: move this to Notations *)
-Reserved Notation "'slet' x .. y <- X ; B"
-         (at level 200, x binder, y binder, B at level 200, format "'slet'  x .. y  <-  X  ; '//' B").
-Notation "'slet' x .. y <- X ; B"  := (symex_bind X (fun x => .. (fun y => B%symex) .. )) : symex_scope.
-Notation "A <- X ; B" := (symex_bind X (fun A => B%symex)) : symex_scope.
-(*Infix ";;" := sequence : option_scope.
-Infix ";;;" := sequence_return : option_scope.*)
 
 Definition symex_ident {t} (idc : ident t) : symex_T t.
-  Print IdentifiersBasicGENERATED.Compilers.ident.
-  refine match idc in ident t return symex_T t with
-         | ident.Literal Compilers.Z v
-           => idx <- merge_literalM v;
-                symex_return idx
-         | ident.Z_add
-           => Success (fun x => Success (fun y => x <- x; y <- y; idx <- ?[merge_addition] x y; symex_return idx))
-         | _ => ltac:(shelve)
-         end%symex; cbn.
-Admitted.
+Proof.
+  refine (let symex_mod_zrange idx range := symex_error (Unhandled_identifier idc) in
+          match idc in ident t return symex_T t with
+          | ident.Literal base.type.Z v
+            => idx <- merge_literalM v;
+               symex_return idx
 
-Fixpoint symex_expr {t} (e : API.expr (var:=var) t) : symex_T t.
-  refine match e in expr.expr t return symex_T t with
+          | ident.Z_add
+            => fun x y => idx <- merge_addition x y; symex_return idx
+
+          | ident.Z_modulo
+          | ident.Z_mul
+          | ident.Z_pow
+          | ident.Z_sub
+          | ident.Z_opp
+          | ident.Z_div
+          | ident.Z_log2
+          | ident.Z_log2_up
+          | ident.Z_to_nat
+          | ident.Z_shiftr
+          | ident.Z_shiftl
+          | ident.Z_land
+          | ident.Z_lor
+          | ident.Z_min
+          | ident.Z_max
+          | ident.Z_mul_split
+          | ident.Z_mul_high
+          | ident.Z_add_get_carry
+          | ident.Z_add_with_carry
+          | ident.Z_add_with_get_carry
+          | ident.Z_sub_get_borrow
+          | ident.Z_sub_with_get_borrow
+          | ident.Z_ltz
+          | ident.Z_zselect
+          | ident.Z_add_modulo
+          | ident.Z_truncating_shiftl
+          | ident.Z_bneg
+          | ident.Z_lnot_modulo
+          | ident.Z_lxor
+          | ident.Z_rshi
+          | ident.Z_cc_m
+          | ident.Z_combine_at_bitwidth
+            => symex_T_error (Unhandled_identifier idc)
+
+          | ident.comment _
+          | ident.comment_no_keep _
+            => fun _ => symex_return tt
+          | ident.value_barrier
+            => fun v => symex_return v
+          | ident.Literal base.type.bool _
+          | ident.Literal base.type.string _
+          | ident.tt
+          | ident.None _
+            => symex_return tt
+          | ident.Literal base.type.zrange v
+          | ident.Literal base.type.nat v
+            => symex_return v
+          | ident.Some _
+            => fun _ => symex_return tt
+          | ident.pair _ _
+            => fun a b => symex_return (a, b)
+          | ident.fst _ _
+            => fun a => symex_return (fst a)
+          | ident.snd _ _
+            => fun a => symex_return (snd a)
+          | ident.nil _
+            => symex_return []
+          | ident.cons _
+            => fun x xs => symex_return (x :: xs)
+          | ident.Nat_succ as idc
+          | ident.Nat_pred as idc
+            => fun v => symex_return (ident.interp idc v)
+          | ident.Nat_max as idc
+          | ident.Nat_mul as idc
+          | ident.Nat_add as idc
+          | ident.Nat_sub as idc
+          | ident.List_seq as idc
+            => fun a b => symex_return (ident.interp idc a b)
+          | ident.List_nth_default _
+          | ident.eager_List_nth_default _
+            => fun default ls n => symex_return (List.nth_default default ls n)
+          | ident.List_length _
+            => fun ls => symex_return (List.length ls)
+          | ident.List_firstn _
+            => fun n ls => symex_return (List.firstn n ls)
+          | ident.List_skipn _
+            => fun n ls => symex_return (List.skipn n ls)
+          | ident.List_repeat _
+            => fun v n => symex_return (List.repeat v n)
+          | ident.List_combine _ _
+            => fun ls1 ls2 => symex_return (List.combine ls1 ls2)
+          | ident.List_app _
+            => fun ls1 ls2 => symex_return (List.app ls1 ls2)
+          | ident.List_rev _
+            => fun ls => symex_return (List.rev ls)
+          | ident.Build_zrange (* do we need to handle this? *)
+            => fun l r => symex_error (Unhandled_identifier idc)
+          (* we should handle these the same way that we handle truncation/modulo *)
+          | ident.Z_cast
+            => fun r v_idx => idx <- symex_mod_zrange v_idx r; symex_return idx
+          | ident.Z_cast2
+            => fun '(r1, r2) '(v1_idx, v2_idx)
+               => idx1 <- symex_mod_zrange v1_idx r1;
+                  idx2 <- symex_mod_zrange v2_idx r2;
+                  symex_return (idx1, idx2)
+          | ident.Z_of_nat
+            => fun n => idx <- merge_literalM (Z.of_nat n); symex_return idx
+
+          | ident.Z_eqb
+          | ident.Z_leb
+          | ident.Z_ltb
+          | ident.Z_geb
+          | ident.Z_gtb
+
+          | ident.Nat_eqb
+          | ident.prod_rect _ _ _
+          | ident.bool_rect _
+          | ident.bool_rect_nodep _
+          | ident.nat_rect _
+          | ident.eager_nat_rect _
+          | ident.nat_rect_arrow _ _
+          | ident.eager_nat_rect_arrow _ _
+          | ident.list_rect _ _
+          | ident.eager_list_rect _ _
+          | ident.list_rect_arrow _ _ _
+          | ident.eager_list_rect_arrow _ _ _
+          | ident.list_case _ _
+          | ident.List_map _ _
+          | ident.List_flat_map _ _
+          | ident.List_partition _
+          | ident.List_fold_right _ _
+          | ident.List_update_nth _
+          | ident.option_rect _ _
+          | ident.zrange_rect _
+          | ident.fancy_add
+          | ident.fancy_addc
+          | ident.fancy_sub
+          | ident.fancy_subb
+          | ident.fancy_mulll
+          | ident.fancy_mullh
+          | ident.fancy_mulhl
+          | ident.fancy_mulhh
+          | ident.fancy_rshi
+          | ident.fancy_selc
+          | ident.fancy_selm
+          | ident.fancy_sell
+          | ident.fancy_addm
+            => symex_T_error (Unhandled_identifier idc)
+          end%symex).
+  all: cbn.
+Defined.
+
+Fixpoint symex_expr {t} (e : API.expr (var:=var) t) : symex_T t
+  := match e in expr.expr t return symex_T t with
      | expr.Ident _ idc => symex_ident idc
      | expr.Var _ v => symex_T_return v
-     | expr.Abs _ _ f => Success _
-     | expr.App _ _ f x
+     | expr.Abs (type.base _) _ f => fun v => @symex_expr _ (f v)
+     | expr.App (type.base _) _ f x
        => let ef := @symex_expr _ f in
           let ex := @symex_expr _ x in
-          _
-          (*ef ex*)
-     | expr.LetIn _ _ x f
-       => let ef := (*@symex_expr _ f*)_ in
+          symex_T_bind_base ex ef
+     | expr.LetIn (type.base _) _ x f
+       => let ef v := @symex_expr _ (f v) in
           let ex := @symex_expr _ x in
-          _
-         end%symex; cbn in *; fold symex_T.
-
-  shelve.
-  fold symex_T.
-  shelve.
-Admitted.
+          symex_T_bind_base ex ef
+     | expr.App (type.arrow _ _) _ f x
+       => symex_T_error (Invalid_higher_order_application f x)
+     | expr.LetIn (type.arrow _ _) _ x f
+       => symex_T_error (Invalid_higher_order_let x)
+     | expr.Abs (type.arrow _ _) _ _
+       => fun v : Empty_set => match v with end
+     end.
 
 Section check_equivalence.
   Context {assembly_calling_registers' : assembly_calling_registers_opt}
@@ -334,7 +498,6 @@ Section check_equivalence.
           let d := empty_dag in
           let gensym_st := gensym_state_init in
           input_types <- simplify_input_type t arg_bounds;
-          output_types <- simplify_base_type (type.final_codomain t) out_bounds;
           let '(inputs, (d, gensym_st)) := build_inputs (d, gensym_st) input_types in
           input_var_data <- build_input_var t inputs;
           let '(input_var_data, unused_inputs) := input_var_data in
@@ -343,34 +506,10 @@ Section check_equivalence.
               := invert_expr.smart_App_curried (expr _) input_var_data in
           symevaled_PHOAS <- symex_expr ast d;
           let '(PHOAS_output, PHOAS_dag) := symevaled_PHOAS in
+          let stack_size : nat := N.to_nat (assembly_stack_size asm) in
+          output_types <- simplify_base_type (type.final_codomain t) out_bounds;
+          (*let asm_lines : Lines := asm in*)
           _)%error.
-          (* outputs come first, assuming assembly_output_first *)
-          let res := prod_sequence_reg_available
-                       [] assembly_output_first
-                       (fun reg_available => make_output_reg_data reg_available out_bounds)
-                       (fun reg_available => make_input_reg_data reg_available arg_bounds)
-                       reg_available in
-
-          (decl <- match res with
-                   | inl (Success decl, _reg_available) => Success decl
-                   | inl (Error err, _) => Error (Invalid_bounds_data err)
-                   | inr n => Error (Not_enough_registers (List.length reg_available) n)
-                   end;
-           let '(output_registers, input_registers) := decl in
-           (* we now construct the inputs to the equivalence checker:
-              - the list of registers and array sizes for outputs
-              - the list of registers and array sizes for inputs
-              - the stack size
-              - the expression specialized to some appropriate variable type
-              - the assembly expression is available in the context as asm *)
-           let output_register_list : list (REG * nat) := reg_list_of_base_reg_data output_registers in
-           let input_register_list : list (REG * nat) := reg_list_of_input_reg_data input_registers in
-           let stack_size : nat := N.to_nat (assembly_stack_size asm) in
-           let ast : API.expr (type.base (type.final_codomain t))
-               := invert_expr.smart_App_curried (expr _) (type.map_for_each_lhs_of_arrow (@reg_data_to_var) input_registers) in
-           let asm_lines : Lines := asm in
-
-           _)%error).
       refine (if false
               then Success tt
               else Error Could_not_prove_equivalence).
